Day 16, part 1

Day16.lean
@@ -83,26 +83,26 @@ private def OpticsElement.outputDirections : OpticsElement → EnterDirection �
 | OpticsElement.Splitter SplitterDirection.Vertical, EnterDirection.FromBottom => [ExitDirection.ToTop]
 | OpticsElement.Splitter SplitterDirection.Vertical, EnterDirection.FromRight => [ExitDirection.ToTop, ExitDirection.ToBottom]
 
-private def OpticsTable.neighbour? {table : OpticsTable} (outDirection : ExitDirection) (coordinate : table.Coordinate) : Option table.Coordinate :=
+private def OpticsTable.neighbour? {table : OpticsTable} (outDirection : ExitDirection) (coordinate : table.Coordinate) : Option (EnterDirection × table.Coordinate) :=
   match outDirection with
   | ExitDirection.ToBottom =>
     if h : coordinate.y.succ < table.height then
-      some {coordinate with y := ⟨coordinate.y.succ, h⟩}
+      some (EnterDirection.FromTop, {coordinate with y := ⟨coordinate.y.succ, h⟩})
     else
       none
   | ExitDirection.ToLeft =>
     if 0 < coordinate.x.val then
-      some {coordinate with x := ⟨coordinate.x.val.pred,Nat.lt_of_le_of_lt (Nat.pred_le _) coordinate.x.isLt⟩}
+      some (EnterDirection.FromRight,{coordinate with x := ⟨coordinate.x.val.pred,Nat.lt_of_le_of_lt (Nat.pred_le _) coordinate.x.isLt⟩})
     else
       none
   | ExitDirection.ToTop =>
     if 0 < coordinate.y.val then
-      some {coordinate with y := ⟨coordinate.y.val.pred, Nat.lt_of_le_of_lt (Nat.pred_le _) coordinate.y.isLt⟩}
+      some (EnterDirection.FromBottom, {coordinate with y := ⟨coordinate.y.val.pred, Nat.lt_of_le_of_lt (Nat.pred_le _) coordinate.y.isLt⟩})
     else
       none
   | ExitDirection.ToRight =>
     if h : coordinate.x.succ < table.width then
-      some {coordinate with x := ⟨coordinate.x.succ, h⟩}
+      some (EnterDirection.FromLeft, {coordinate with x := ⟨coordinate.x.succ, h⟩})
     else
       none
 
@@ -118,15 +118,82 @@ private def SeenExitDirection.setRight : SeenExitDirection → SeenExitDirection
 private def SeenExitDirection.setBottom : SeenExitDirection → SeenExitDirection := BitVec.setBitTrue 2
 private def SeenExitDirection.setLeft : SeenExitDirection → SeenExitDirection := BitVec.setBitTrue 3
 
+private def SeenExitDirection.contains (d : SeenExitDirection) : ExitDirection → Bool
+| ExitDirection.ToTop => d.top
+| ExitDirection.ToRight => d.right
+| ExitDirection.ToBottom => d.bottom
+| ExitDirection.ToLeft => d.left
+
+private def SeenExitDirection.setDirection (d : SeenExitDirection) : ExitDirection → SeenExitDirection
+| ExitDirection.ToTop => d.setTop
+| ExitDirection.ToRight => d.setRight
+| ExitDirection.ToBottom => d.setBottom
+| ExitDirection.ToLeft => d.setLeft
+
+instance : ToString SeenExitDirection where
+  toString := λc ↦
+  match h : c with
+  | 0b0000#4 => "."
+  | 0b0001#4 => "↑"
+  | 0b0010#4 => "→"
+  | 0b0011#4 => "└"
+  | 0b0100#4 => "↓"
+  | 0b0101#4 => "↕"
+  | 0b0110#4 => "┌"
+  | 0b0111#4 => "├"
+  | 0b1000#4 => "←"
+  | 0b1001#4 => "┘"
+  | 0b1010#4 => "↔"
+  | 0b1011#4 => "┴"
+  | 0b1100#4 => "┐"
+  | 0b1101#4 => "┤"
+  | 0b1110#4 => "┬"
+  | 0b1111#4 => "┼"
+  | ⟨x+16,_⟩ =>
+    -- above Fin 15 exhaustive matches are not auto-detected, see https://github.com/leanprover/lean4/issues/5181 and Contradiction.Config.searchFuel
+    False.elim (absurd c.isLt (Nat.not_lt_of_ge $ h.substr $ Nat.le_add_left 16 x))
+
 private def SeenExitDirection.countDirection (a : SeenExitDirection) : Fin 5 :=
   ⟨
     a.top.toNat + a.right.toNat + a.bottom.toNat + a.left.toNat,
     Nat.lt_succ_of_le $ Nat.add_le_add (Nat.add_le_add (Nat.add_le_add (Bool.toNat_le _) (Bool.toNat_le _)) (Bool.toNat_le _)) (Bool.toNat_le _)
   ⟩
 
+private def SeenExitDirection.isEnergized : SeenExitDirection → Bool
+| 0b0000#4 => false
+| _ => true
+
+private theorem SeenExitDirection.setDirection_increasesCountDirection (a : SeenExitDirection) (e : ExitDirection) (h₁ : a.contains e = false) : a.countDirection < (a.setDirection e).countDirection := by
+  have Fin.val_three : ∀(n : Nat), (3 : Fin (n + 4)).val = 3 := λx↦rfl
+  cases e
+  all_goals
+    unfold contains at h₁
+    simp[countDirection, setDirection, setTop, setLeft, setRight, setBottom, left, right, bottom, top] at h₁ ⊢
+    simp[h₁, BitVec.setBitTrue, Fin.val_three]
+    unfold getElem BitVec.instGetElemNatBoolLt BitVec.getLsb' Nat.testBit
+    simp
+
 private structure SeenExitDirections (table : OpticsTable) extends Parsing.RectangularGrid SeenExitDirection where
   sameWidth : width = table.width
   sameHeight : height = table.height
+
+instance {table : OpticsTable} : ToString (SeenExitDirections table) where
+  toString := λes ↦ Id.run do
+  let mut result := ""
+  for hl: line in [:es.height] do
+    for hc: column in [:es.width] do
+      result := result.append $ ToString.toString (es.toRectangularGrid[{x := ⟨column, hc.upper⟩, y := ⟨line, hl.upper⟩ : es.Coordinate}])
+    result := result.append "\n"
+  result
+
+instance {table : OpticsTable} : Repr (SeenExitDirections table) where
+  reprPrec t _ := ToString.toString t
+
+private def SeenExitDirections.set {table : OpticsTable} {d : SeenExitDirections table} (c : d.Coordinate) (v : SeenExitDirection) : SeenExitDirections table :=
+  {
+    d with
+      toRectangularGrid := d.toRectangularGrid.set c v
+  }
 
 private def SeenExitDirections.empty (table : OpticsTable) : SeenExitDirections table :=
   {
@@ -171,17 +238,122 @@ private def SeenExitDirections.countExitDirections {table : OpticsTable} (seenDi
     rw[seenDirections.sameHeight, seenDirections.sameWidth]
   Fin.cast h₂.symm ⟨c,Nat.lt_succ_of_le h₁⟩
 
+/-- Factored out to work around that annoying "generalize failed, result is not type correct" errror -/
+private theorem SeenExitDirections.countExitDirections_increasesWhenSet_Aux (l : List SeenExitDirection) (i : Nat) (h₁ : i < l.length) (direction : ExitDirection) (h₂ : l[i].contains direction = false) (prev: Nat) : List.foldl (fun n e => n + e.countDirection.val) prev l < List.foldl (fun n e => n + e.countDirection.val) prev (l.set i (l[i].setDirection direction)) := by
+  cases i
+  case zero =>
+    unfold List.set
+    split; case h_2 | h_3 => contradiction
+    case h_1 r1 r2 r3 d ds r4 =>
+      clear r1 r2 r3 r4
+      simp at h₂ ⊢
+      simp only [←List.foldl_map]
+      rewrite[Nat.add_comm]
+      rewrite(config:={occs := .pos [2]})[Nat.add_comm]
+      simp[List.foldl_assoc]
+      -- f-ing finally
+      exact SeenExitDirection.setDirection_increasesCountDirection _ _ h₂
+  case succ j =>
+    match l with
+    | a :: as =>
+      simp at h₁ h₂ ⊢
+      apply countExitDirections_increasesWhenSet_Aux
+      assumption
+
+private theorem SeenExitDirections.countExitDirections_increasesWhenSet {table : OpticsTable} (seenDirections : SeenExitDirections table) (index : seenDirections.Coordinate) (direction : ExitDirection) (h₁ : seenDirections.toRectangularGrid[index].contains direction = false) : (seenDirections.countExitDirections) < (seenDirections.set index $ seenDirections.toRectangularGrid[index].setDirection direction).countExitDirections := by
+  unfold countExitDirections SeenExitDirections.set Parsing.RectangularGrid.set getElem Parsing.instGetElemRectangularGridCoordinateEq Parsing.RectangularGrid.Get
+  unfold getElem Parsing.instGetElemRectangularGridCoordinateEq Parsing.RectangularGrid.Get at h₁
+  simp at h₁ ⊢
+  unfold Parsing.RectangularGrid.Coordinate.toIndex at h₁ ⊢
+  unfold Array.set
+  simp[Array.foldl_eq_foldl_toList] at h₁ ⊢
+  rw[Array.getElem_eq_getElem_toList] at h₁ ⊢
+  apply countExitDirections_increasesWhenSet_Aux
+  assumption
+
+private def OpticsTable.findFirstExitDirectionNotSeenInQueue {table : OpticsTable} (seenDirections : SeenExitDirections table) (beams : List (EnterDirection × table.Coordinate)) : Option (table.Coordinate × ExitDirection × List (EnterDirection × table.Coordinate)) :=
+  match beams with
+  | [] => none
+  | b :: bs =>
+    let opticsElement := table[b.snd]
+    let outputDirections := opticsElement.outputDirections b.fst
+    let sdCoordinate : seenDirections.Coordinate := {
+      x := Fin.cast seenDirections.sameWidth.symm b.snd.x
+      y := Fin.cast seenDirections.sameHeight.symm b.snd.y
+    }
+    let seenExitDirections := seenDirections.toRectangularGrid[sdCoordinate]
+    let notSeenOutputDirections := outputDirections.filter λd ↦ not $ seenExitDirections.contains d
+    match notSeenOutputDirections with
+    | [] => findFirstExitDirectionNotSeenInQueue seenDirections bs
+    | a :: [] => some (b.snd, a, bs)
+    | a :: _ => some (b.snd, a, b :: bs)
+
+private theorem OpticsTable.findFirstExitDirectionNotSeenInQueue_notContains {table : OpticsTable} (seenDirections : SeenExitDirections table) (beams : List (EnterDirection × table.Coordinate)) {result : table.Coordinate × ExitDirection × List (EnterDirection × table.Coordinate)} (h₁ : OpticsTable.findFirstExitDirectionNotSeenInQueue seenDirections beams = some result) : seenDirections.toRectangularGrid[{x := Fin.cast seenDirections.sameWidth.symm result.fst.x, y := Fin.cast seenDirections.sameHeight.symm result.fst.y : seenDirections.Coordinate}].contains result.snd.fst = false := by
+  unfold findFirstExitDirectionNotSeenInQueue at h₁
+  split at h₁
+  case h_1 => contradiction
+  case h_2 del b bs =>
+    clear del
+    simp at h₁
+    split at h₁
+    case h_1 =>
+      exact findFirstExitDirectionNotSeenInQueue_notContains seenDirections bs h₁
+    case' h_2 ed heq | h_3 ed eds _ heq =>
+      have h₂ := Option.some.inj h₁
+      subst result
+      generalize { x := Fin.cast _ b.snd.x, y := Fin.cast _ b.snd.y : seenDirections.Coordinate } = c at *
+      have h₂ : ed ∈ List.filter (fun d => !seenDirections.toRectangularGrid[c].contains d) (OpticsElement.outputDirections table[b.snd] b.fst) := by simp only [heq, List.mem_singleton, List.mem_cons, true_or]
+      exact (Bool.not_eq_true' _).mp (List.mem_filter.mp h₂).right
+
 private def OpticsTable.followPath {table : OpticsTable} (seenDirections : SeenExitDirections table) (beams : List (EnterDirection × table.Coordinate)) : SeenExitDirections table :=
   -- step 1: discard all beams from the beginning of the list
   --         that do not yield at least one not-yet-seen exit-direction.
   -- step 2a: if no beams are left, done.
   -- step 2: for the first beam that yields new exit directions,
-  --         add those exit directions at the end of the beams list and
+  --         add those exit directions at the start of the beams list and
   --         mark them as seen.
   -- step 3: recurse
   -- step 4: profit
+  match _h₁ : table.findFirstExitDirectionNotSeenInQueue seenDirections beams with
+  | none => seenDirections
+  | some (coordinate, exitDirection, remainingBeams) =>
+    let sdCoordinate : seenDirections.Coordinate := {
+      x := Fin.cast seenDirections.sameWidth.symm coordinate.x
+      y := Fin.cast seenDirections.sameHeight.symm coordinate.y
+    }
+    let newSeenDirections := seenDirections.set sdCoordinate
+      (seenDirections.toRectangularGrid[sdCoordinate].setDirection exitDirection)
+    match table.neighbour? exitDirection coordinate with
+    | none =>
+      -- no neighbour, but we still need to note down the exit direction as seen
+      OpticsTable.followPath newSeenDirections remainingBeams
+    | some cd =>
+      OpticsTable.followPath newSeenDirections (cd :: remainingBeams)
+termination_by 4 * table.width * table.height - seenDirections.countExitDirections
+decreasing_by
+  all_goals
+  apply Nat.sub_lt_of_gt
+  case h₁ =>
+    exact Nat.le_of_lt_succ $ Fin.isLt _
+  case h₂ =>
+    apply SeenExitDirections.countExitDirections_increasesWhenSet
+    exact OpticsTable.findFirstExitDirectionNotSeenInQueue_notContains seenDirections beams _h₁
 
-  sorry
+private def SeenExitDirections.countEnergizedTiles {table : OpticsTable} (seenDirections : SeenExitDirections table) : Nat :=
+  seenDirections.elements.foldl (λc ed ↦ c + ed.isEnergized.toNat) 0
+
+def part1 (table : OpticsTable) : Nat :=
+  let seenDirections := table.followPath (SeenExitDirections.empty table) [(EnterDirection.FromLeft, {x := ⟨0,table.not_empty.left⟩, y := ⟨0,table.not_empty.right⟩})]
+  seenDirections.countEnergizedTiles
+
+
+------------------------------------------------------------------------------------
+open DayPart
+instance : Parse ⟨16, by simp⟩ (ι := OpticsTable) where
+  parse := (Except.mapError ToString.toString) ∘ parse
+
+instance : Part ⟨16,_⟩ Parts.One (ι := OpticsTable) (ρ := Nat) where
+  run := λc ↦ some (part1 c)
 
 ------------------------------------------------------------------------------------
 
@@ -198,3 +370,12 @@ private def testInput := r".|...\....
 ..//.|...."
 
 #eval parse testInput
+
+#eval match parse testInput with
+| Except.error e => s!"Error: {e}".toFormat
+| Except.ok ot =>
+  Repr.reprPrec (ot.followPath (SeenExitDirections.empty ot) [(EnterDirection.FromLeft, {x := ⟨0,ot.not_empty.left⟩, y := ⟨0,ot.not_empty.right⟩})]) 0
+
+#eval match parse testInput with
+| Except.error e => s!"Error: {e}"
+| Except.ok ot => ToString.toString $ part1 ot
